monads/typeclasses/Monad.v
@@ -1,36 +1,49 @@
-Require Import Coq.Logic.FunctionalExtensionality.
-Require Import Coq.Program.Basics.
+Require Import FunctionalExtensionality Program Setoid.
 
 Set Implicit Arguments.
 
 Local Open Scope program_scope.
 
 Class Monad (m : Type -> Type)
+            (mequiv : forall {T : Type}, m T -> m T -> Prop)
             (ret : forall {A : Type}, A -> m A)
             (bind : forall {A B : Type}, m A -> (A -> m B) -> m B) : Prop := {
   (** Three laws that a monad instance must obey.
     Law 1:  return x >>= f ~ f x
     Law 2:  m >>= return ~ m
     Law 3:  (m >>= f) >>= g ~ m >>= (fun x -> f x >>= g) *)
-  left_id : forall (A B : Type) (x : A) (f : A -> m B),
-           bind (ret x) f = f x;
+  left_id :
+    forall (A B : Type) (x : A) (f : A -> m B),
+      mequiv (bind (ret x) f) (f x);
 
-  right_id : forall (A : Type) (x : m A),
-           bind x ret = x;
+  right_id :
+    forall (A : Type) (x : m A),
+      mequiv (bind x ret) x;
 
-  bind_assoc : forall (A B C : Type) (n : m A) (f : A -> m B) (g : B -> m C),
-           bind (bind n f) g = bind n (fun x => bind (f x) g);
+  bind_assoc :
+    forall (A B C : Type) (n : m A) (f : A -> m B) (g : B -> m C),
+      mequiv (bind (bind n f) g) (bind n (fun x => bind (f x) g));
+
+  equivalence :
+    forall T, Equivalence (@mequiv T);
+
+  f_equivalence :
+    forall {A B : Type} n (f g : A -> m B),
+      (forall x, mequiv (f x) (g x)) -> mequiv (bind n f) (bind n g);
 }.
 
 Section MonadProperties.
-  Generalizable Variables m ret bind.
+  Generalizable All Variables.
+  Context `{Monad m mequiv ret bind}.
 
-  Variable m : Type -> Type.
-  Variable ret : forall {A : Type}, A -> m A.
-  Variable bind : forall {A B : Type}, m A -> (A -> m B) -> m B.
-  Variable monad : Monad m ret bind.
-
+  Infix "=~" := mequiv (at level 60, no associativity).
   Infix ">>=" := bind (at level 50, left associativity).
+
+  Instance mequivEquivlence :
+    forall T, Equivalence (@mequiv T).
+  Proof.
+    apply equivalence.
+  Qed.
 
   Definition fmap {A B : Type} (f : A -> B) (n : m A) : m B :=
     n >>= (@ret B) ∘ f.
@@ -38,75 +51,76 @@ Section MonadProperties.
   Definition join {A : Type} (n : m (m A)) : m A :=
     n >>= id.
 
+  Ltac revealer := unfold join, fmap, compose, id; intros.
+  Ltac f_equal := apply f_equivalence; intros.
+
   Theorem fmap_compose_join_eq_bind :
     forall (A B : Type) (n : m A) (f : A -> m B),
-      n >>= f = join (fmap f n).
+      n >>= f =~ join (fmap f n).
   Proof.
-    unfold join, fmap; intros.
-    rewrite bind_assoc.
-    f_equal; apply functional_extensionality; intros.
-    unfold compose; rewrite left_id.
-    auto.
+    revealer.
+    rewrite bind_assoc. f_equal.
+    rewrite left_id. reflexivity.
   Qed.
 
   (** Properties for Monad as a Functor. *)
   Theorem fmap_id :
-    forall (A : Type), fmap (@id A) = @id (m A).
+    forall (A : Type) (n : m A),
+      fmap id n =~ n.
   Proof.
-    unfold fmap, compose; intros.
-    apply functional_extensionality; intros; unfold id.
-    rewrite right_id. auto.
+    revealer.
+    rewrite right_id. reflexivity.
   Qed.
 
   Theorem fmap_associativity :
-    forall (A B C : Type) (f : A -> B) (g : B -> C),
-      fmap (g ∘ f) = fmap g ∘ fmap f.
+    forall (A B C : Type) (f : A -> B) (g : B -> C) (n : m A),
+      fmap (g ∘ f) n =~ fmap g (fmap f n).
   Proof.
-    unfold fmap, compose; intros.
-    apply functional_extensionality; intros.
-    rewrite bind_assoc; f_equal.
-    apply functional_extensionality; intros.
-    rewrite left_id. auto.
+    revealer.
+    rewrite bind_assoc. f_equal.
+    rewrite left_id. reflexivity.
   Qed.
 
   (** https://en.wikipedia.org/wiki/Monad_(functional_programming)#fmap_and_join *)
   Theorem return_property :
     forall (A B : Type) (f : A -> B) (x : A),
-      ret (f x) = fmap f (ret x).
+      ret (f x) =~ fmap f (ret x).
   Proof.
-    unfold fmap, compose; intros.
-    rewrite left_id. auto.
+    revealer.
+    rewrite left_id. reflexivity.
   Qed.
 
   Theorem join_property1 :
     forall (A : Type) (x : m (m (m A))),
-      join (fmap join x) = join (join x).
+      join (fmap join x) =~ join (join x).
   Proof.
     intros. rewrite <- fmap_compose_join_eq_bind.
-    unfold join, id. rewrite bind_assoc. auto.
+    revealer.
+    rewrite bind_assoc. reflexivity.
   Qed.
 
   Theorem join_property2 :
     forall (A : Type) (x : m A),
-      join (fmap (@ret A) x) = x.
+      join (fmap (@ret A) x) =~ x.
   Proof.
     intros. rewrite <- fmap_compose_join_eq_bind.
-    rewrite right_id. auto.
+    rewrite right_id. reflexivity.
   Qed.
 
   Theorem join_property3 :
     forall (A : Type) (x : m A),
-      join (ret x) = x.
+      join (ret x) =~ x.
   Proof.
-    intros. unfold join.
-    rewrite left_id. auto.
+    revealer.
+    rewrite left_id. reflexivity.
   Qed.
 
   Theorem join_property4 :
     forall (A B : Type) (f : A -> B) (x : m (m A)),
-      join (fmap (fmap f) x) = fmap f (join x).
+      join (fmap (fmap f) x) =~ fmap f (join x).
   Proof.
     intros. rewrite <- fmap_compose_join_eq_bind.
-    unfold fmap, join. rewrite bind_assoc. auto.
+    revealer.
+    rewrite bind_assoc. reflexivity.
   Qed.
 End MonadProperties.
