monads/typeclasses/Free.v
@@ -1,0 +1,72 @@
+(** Idea comes from https://github.com/tchajed/coq-io *)
+
+(** Verifying free monad is a monad. *)
+
+Require Import Arith RelationClasses.
+Require Import Monads.Monad.
+Require Import Tactics.CpdtTactics.
+
+Set Implicit Arguments.
+
+Module Heap.
+  Definition heap := nat -> option nat.
+
+  Definition empty : heap := fun _ => None.
+
+  Definition add (m : heap) (k : nat) (v : nat) : heap :=
+    fun k' => if (k' =? k) then Some v else m k'.
+  Definition lookup (m : heap) (k : nat) : option nat := m k.
+End Heap.
+
+Import Heap.
+
+Inductive cmd : Type -> Type :=
+| Return (A : Type) (r : A) : cmd A
+| Bind (A B : Type) (c1 : cmd A) (c2 : A -> cmd B) : cmd B
+| Read (p : nat) : cmd nat
+| Write (p v : nat) : cmd unit.
+
+Inductive execute : forall (A : Type), heap -> cmd A -> heap -> A -> Prop :=
+| ExeReturn :
+    forall A h (x : A),
+      execute h (Return x) h x
+| ExeBind :
+    forall A B (c1 : cmd A) (c2 : A -> cmd B) h1 h2 h3 x y,
+      execute h1 c1 h2 x ->
+      execute h2 (c2 x) h3 y ->
+      execute h1 (Bind c1 c2) h3 y
+| ExeRead :
+    forall h p v,
+      lookup h p = Some v ->
+      execute h (Read p) h v
+| ExeWrite :
+    forall h p v,
+      execute h (Write p v) (add h p v) tt.
+
+Hint Constructors execute.
+
+Definition execute_equiv {A : Type} (c1 c2 : cmd A) :=
+  (forall h1 h2 v, execute h1 c1 h2 v -> execute h1 c2 h2 v) /\
+  (forall h1 h2 v, execute h1 c2 h2 v -> execute h1 c1 h2 v).
+
+Instance execute_equiv_Equivalence :
+  forall (A : Type), Equivalence (@execute_equiv A).
+Proof.
+  unfold execute_equiv; constructor; hnf; intuition.
+Qed.
+
+Hint Resolve execute_equiv_Equivalence.
+
+Ltac solver :=
+  repeat match goal with
+         | [ H: execute _ (Return _) _ _ |- _ ] =>
+             inversion H; subst; clear H
+         | [ H: execute _ (Bind _ _) _ _ |- _ ] =>
+             inversion H; subst; clear H
+         end; crush.
+
+Instance free_monad : Monad cmd (@execute_equiv) Return Bind.
+Proof.
+  split; intros; intuition; unfold execute_equiv in *; intuition;
+  repeat solver; econstructor; eauto; specialize (H x); intuition.
+Qed.
